theories/vprop.v
@@ -1,0 +1,23 @@
+(* In this file we define [vProp], the type of propositions in the high-level
+logic. *)
+
+From iris.bi Require Export monpred big_op.
+From iris.proofmode Require Import tactics monpred modality_instances.
+From iris.base_logic.lib Require Import fancy_updates.
+
+From self Require Import view.
+
+(* We define a canonical [biIndex] structure for [view]. All fields except for
+[bi_index_type] can be infered by Coq. *)
+Canonical Structure view_bi_index : biIndex :=
+  {| bi_index_type := view |}.
+
+(* Uncomment this to see the fields that Coq infer. *)
+(* Print view_bi_index. *)
+
+Instance view_bi_index_bot (V : view) : BiIndexBottom ∅ := view_empty_least.
+
+(* Types of view predicates. *)
+Definition vProp Σ := monPred view_bi_index (uPredI (iResUR Σ)). (* FIXME: use iPropI here. *)
+Definition vPropO Σ := monPredO view_bi_index (uPredI (iResUR Σ)).
+Definition vPropI Σ := monPredI view_bi_index (uPredI (iResUR Σ)).
