theories/weakestpre.v
@@ -1,0 +1,53 @@
+(* In this file we define our weakest precondition on top of the weakest
+(* precondition included in Iris. *) *)
+
+From iris.proofmode Require Export tactics.
+From iris.algebra Require Import gmap excl auth.
+From iris.program_logic Require weakestpre.
+From iris.program_logic Require Import ownp.
+
+From self Require Import vprop view lang.
+From self.lang Require Import primitive_laws syntax.
+
+Section wp.
+  Context `{!nvmG Σ}.
+
+  Implicit Types (Φ : val → vProp Σ) (e : expr).
+  (* (P Q : vProp Σ) (E : coPset) *)
+
+  (* Our weakest precondition is a [vProp]. We construct it using [MonPred]
+  which wraps the function along with a proof that it is monotone. *)
+  Program Definition wp_def s E e Φ : vProp Σ :=
+    MonPred (λ V,
+      ∀ TV, ⌜V ⊑ TV.(tv_store_view)⌝ -∗
+            valid (TV.(tv_store_view)) -∗
+            WP (ThreadState e TV) @ s; E {{ λ '(ThreadVal v TV), (Φ v (TV.(tv_store_view))) }})%I%V _.
+  Next Obligation. solve_proper. Qed.
+
+  (* This is sealing follows the same ritual as the [wp] in Iris. *)
+  Definition wp_aux : seal (@wp_def). by eexists. Qed.
+
+  Global Instance expr_wp : Wp expr_lang (vProp Σ) stuckness := unseal (wp_aux).
+
+  Lemma wp_eq : wp = wp_def.
+  Proof. rewrite -wp_aux.(seal_eq). done. Qed.
+
+  (* We prove a few basic facts about our weakest precondition. *)
+  Global Instance wp_ne s E e n :
+    Proper (pointwise_relation _ (dist n) ==> dist n) (wp s E e).
+  Proof. rewrite wp_eq. split=>V. Admitted. (* solve_proper. Qed. *) (* FIXME: Why does this not work? *)
+  Global Instance wp_proper s E e :
+    Proper (pointwise_relation val (≡) ==> (≡)) (wp s E e).
+  Proof. rewrite wp_eq. constructor=>V.
+    (* solve_proper. Qed. *)
+  Admitted.
+
+  (* If the expression is a value then showing the postcondition for the value
+  suffices. *)
+  Lemma wp_value E Φ v : Φ v ⊢ WP (of_val v) @ E {{ Φ }}.
+  Proof.
+    iStartProof (iProp _). simpl. rewrite wp_eq /wp_def. iIntros "% HΦ %% ?".
+    iApply (wp_value' _ _ _ (ThreadVal v _)). iFrame.
+  Qed.
+
+End wp.
